Erase application, now featuring dependent heaven/hell

LeanToLambdaBox/Contexts.lean
@@ -16,8 +16,21 @@ end Extension
 private def MultiExtension (ctx ctx': GenericSizedContext): Prop := ctx ≤ ctx'
 namespace MultiExtension
 private def trivial: MultiExtension ctx ctx := Nat.le_refl _
+private def compose: (ext: MultiExtension ctx ctx') -> (ext': MultiExtension ctx' ctx'') -> MultiExtension ctx ctx'' := Nat.le_trans
+private def weakenId: MultiExtension ctx ctx' -> ctx.Id -> ctx'.Id := Fin.castLE
 end MultiExtension
 end GenericSizedContext
+
+private theorem list_index_cast { l' l: List α } (eq: l' = l) (i: Fin (l.length)): l'[Fin.cast (congrArg List.length eq).symm i] = l[i] := by
+  cases eq
+  rfl
+
+private theorem length_le_length_append {as bs: List α}: as.length ≤ (as ++ bs).length := by
+  rewrite [List.length_append]
+  apply Nat.le_add_right
+
+private theorem getElem_append_left_fin (as bs: List α) (i: Fin as.length) (h: as.length <= (as ++ bs).length): (as ++ bs)[Fin.castLE h i] = as[i] := by
+  apply List.getElem_append_left
 
 private abbrev GenericArrayContext α := Array α
 namespace GenericArrayContext
@@ -30,6 +43,30 @@ private def Extension (ctx ctx': GenericArrayContext α) (x: α): Prop := ctx' =
 private def MultiExtension (ctx ctx': GenericArrayContext α): Prop := ctx.toList.IsPrefix ctx'.toList
 namespace MultiExtension
 private def trivial: MultiExtension ctx ctx := ⟨[], List.append_nil _⟩
+private def compose (ext: MultiExtension ctx ctx') (ext': MultiExtension ctx' ctx''): MultiExtension ctx ctx'' := by
+  cases ext with | intro l h =>
+  cases ext' with | intro l' h'=>
+  exists l ++ l'
+  rewrite [<-List.append_assoc, h, h']
+  rfl
+
+private def weakenId (ext: MultiExtension ctx ctx'): ctx.Id -> ctx'.Id :=
+  Fin.castLE (by 
+    show ctx.toList.length ≤ ctx'.toList.length
+    cases ext with | intro _ h =>
+    rewrite [<-h]
+    exact length_le_length_append
+  )
+
+private theorem weakenId_getInfo: (@weakenId α ctx ctx' ext i).getInfo = i.getInfo := by
+  let i' := ext.weakenId i
+  cases ext with | intro _ h =>
+  show ctx'.toList[i'] = ctx.toList[i]
+  unfold Id Array.size -- unfolding implicit things in the goal, set pp.explicit to suffer
+  rewrite [<-list_index_cast h i']
+  apply getElem_append_left_fin
+  exact length_le_length_append
+
 end MultiExtension
 end GenericArrayContext
 
@@ -61,7 +98,10 @@ def Extension: (ctx ctx': TypeAliasContext) -> (n: Nat) -> Prop := GenericArrayC
 @[irreducible, local semireducible]
 def MultiExtension: (ctx ctx': TypeAliasContext) -> Prop := GenericArrayContext.MultiExtension
 namespace MultiExtension
+@[irreducible]
 def trivial: MultiExtension ctx ctx := GenericArrayContext.MultiExtension.trivial
+@[irreducible]
+def compose: MultiExtension ctx ctx' -> MultiExtension ctx' ctx'' -> MultiExtension ctx ctx'' := GenericArrayContext.MultiExtension.compose
 end MultiExtension
 end TypeAliasContext
 
@@ -78,25 +118,17 @@ def InductiveContext: Type := GenericArrayContext MutualInductiveSpec
 namespace InductiveContext
 @[irreducible]
 def empty: InductiveContext := GenericArrayContext.empty
-@[irreducible]
-def Extension: (ctx ctx': InductiveContext) -> (spec: MutualInductiveSpec) -> Prop := GenericArrayContext.Extension
-@[irreducible, local semireducible]
-def MultiExtension: (ctx ctx': InductiveContext) -> Prop := GenericArrayContext.MultiExtension
-namespace MultiExtension
-@[irreducible]
-def trivial: MultiExtension ctx ctx := GenericArrayContext.MultiExtension.trivial
-end MultiExtension
 @[irreducible, local semireducible]
 def MutualInductiveId: InductiveContext -> Type := GenericArrayContext.Id
 namespace MutualInductiveId
 @[irreducible]
 def typeFormerArity (mid: MutualInductiveId ctx): Nat := mid.getInfo |>.typeVarCount
-@[irreducible]
+@[irreducible, local semireducible]
 def inductiveArities (mid: MutualInductiveId ctx): List OneInductiveArities := mid.getInfo |>.arities
 @[irreducible, local semireducible]
 def InductiveId (mid: MutualInductiveId ctx): Type := Fin (mid.inductiveArities.length)
 namespace InductiveId
-@[irreducible]
+@[irreducible, local semireducible]
 def constructorArities (iid: @InductiveId ctx mid): List ConstructorArity := mid.inductiveArities |>.get iid
 @[irreducible, local semireducible]
 def ConstructorId (iid: @InductiveId ctx mid): Type := Fin (iid.constructorArities.length)
@@ -108,6 +140,48 @@ end InductiveId
 export InductiveId (ConstructorId)
 end MutualInductiveId
 export MutualInductiveId (InductiveId ConstructorId)
+@[irreducible]
+def Extension: (ctx ctx': InductiveContext) -> (spec: MutualInductiveSpec) -> Prop := GenericArrayContext.Extension
+@[irreducible, local semireducible]
+def MultiExtension: (ctx ctx': InductiveContext) -> Prop := GenericArrayContext.MultiExtension
+namespace MultiExtension
+@[irreducible]
+def trivial: MultiExtension ctx ctx := GenericArrayContext.MultiExtension.trivial
+@[irreducible]
+def compose: MultiExtension ctx ctx' -> MultiExtension ctx' ctx'' -> MultiExtension ctx ctx'' := GenericArrayContext.MultiExtension.compose
+@[irreducible, local semireducible]
+def weakenMutualInductiveId: MultiExtension ctx ctx' -> ctx.MutualInductiveId -> ctx'.MutualInductiveId := GenericArrayContext.MultiExtension.weakenId
+
+theorem weakenMutualInductiveId_inductiveArities : (@weakenMutualInductiveId ctx ctx' ext mid).inductiveArities = mid.inductiveArities := by
+  unfold MutualInductiveId.inductiveArities
+  apply congrArg
+  apply GenericArrayContext.MultiExtension.weakenId_getInfo
+
+unseal InductiveId
+
+@[irreducible, local semireducible]
+def weakenInductiveId (ext: MultiExtension ctx ctx') (iid: @InductiveId ctx mid): (ext.weakenMutualInductiveId mid).InductiveId :=
+  Fin.cast (congrArg List.length weakenMutualInductiveId_inductiveArities).symm iid
+
+theorem weakenInductiveId_constructorArities: (@weakenInductiveId ctx ctx' mid ext iid).constructorArities = iid.constructorArities := by
+  unfold MutualInductiveId.InductiveId.constructorArities
+  unfold InductiveId at iid
+  show (ext.weakenMutualInductiveId mid).inductiveArities[show Fin _ from ext.weakenInductiveId iid] = mid.inductiveArities[iid]
+  exact (list_index_cast weakenMutualInductiveId_inductiveArities iid)
+
+
+unseal ConstructorId
+@[irreducible, local semireducible]
+def weakenConstructorId (ext: MultiExtension ctx ctx') (cid: @ConstructorId ctx mid iid): (ext.weakenInductiveId iid).ConstructorId :=
+  Fin.cast (congrArg List.length weakenInductiveId_constructorArities).symm cid
+
+theorem weakenConstructorId_arity: (@weakenConstructorId ctx ctx' mid iid ext cid).arity = cid.arity := by
+  unfold MutualInductiveId.InductiveId.ConstructorId.arity
+  unfold ConstructorId at cid
+  show (ext.weakenInductiveId iid).constructorArities[show Fin _ from ext.weakenConstructorId cid] = iid.constructorArities[cid]
+  exact (list_index_cast weakenInductiveId_constructorArities cid)
+
+end MultiExtension
 end InductiveContext
 
 structure TypeFormerContext: Type where
@@ -134,7 +208,7 @@ def GlobalValueContext: Type := GenericSizedContext
 namespace GlobalValueContext
 @[irreducible]
 def empty: GlobalValueContext := GenericSizedContext.empty
-@[irreducible]
+@[irreducible, local semireducible]
 def Id: GlobalValueContext -> Type := GenericSizedContext.Id
 @[irreducible]
 def Extension: (ctx ctx': GlobalValueContext) -> Prop := GenericSizedContext.Extension
@@ -143,6 +217,10 @@ def MultiExtension: (ctx ctx': GlobalValueContext)-> Prop := GenericSizedContext
 namespace MultiExtension
 @[irreducible]
 def trivial: MultiExtension ctx ctx := GenericSizedContext.MultiExtension.trivial
+@[irreducible]
+def compose: MultiExtension ctx ctx' -> MultiExtension ctx' ctx'' -> MultiExtension ctx ctx'' := GenericSizedContext.MultiExtension.compose
+@[irreducible]
+def weakenId: MultiExtension ctx ctx' -> ctx.Id -> ctx'.Id := GenericSizedContext.MultiExtension.weakenId
 end MultiExtension
 end GlobalValueContext
 
@@ -173,3 +251,29 @@ def pullback:
   := GenericSizedContext.Extension.pullback
 end Extension
 end LocalValueContext
+
+structure ProgramContext where
+  aliases: TypeAliasContext
+  globals: GlobalValueContext
+  inductives: InductiveContext
+
+namespace ProgramContext
+structure MultiExtension (ctx ctx': ProgramContext) where
+  aliases: ctx.aliases.MultiExtension ctx'.aliases
+  globals: ctx.globals.MultiExtension ctx'.globals
+  inductives: ctx.inductives.MultiExtension ctx'.inductives
+
+namespace MultiExtension
+
+def trivial: MultiExtension ctx ctx where
+  aliases := .trivial
+  globals := .trivial
+  inductives := .trivial
+
+def compose (ext: MultiExtension ctx ctx') (ext': MultiExtension ctx' ctx''): MultiExtension ctx ctx'' where
+  aliases := ext.aliases.compose ext'.aliases
+  globals := ext.globals.compose ext'.globals
+  inductives := ext.inductives.compose ext'.inductives
+
+end MultiExtension
+end ProgramContext
